Clean-up model statements for VM refinement proofs

AxiomaticModels/GenAxiomaticArm.v
@@ -109,6 +109,8 @@ Section Barriers.
 
 End Barriers.
 
+
+(** * Standard names and definitions for Arm axiomatic models *)
 Module AxArmNames.
   Import Candidate.
   Section ArmNames.
@@ -116,27 +118,99 @@ Module AxArmNames.
   Context {et : exec_type} {nmth : nat}.
   Context `(cd : t et nmth).
 
-  Definition F := barriers cd.
+  (** ** Thread relations *)
+  Notation pe := (pre_exec cd).
+  Notation int := (same_thread pe).
+  Notation si := (same_instruction_instance cd).
+  Notation sca := (same_access cd).
+  Notation instruction_order := (instruction_order pe).
+  Notation full_instruction_order := (full_instruction_order pe).
+  Notation iio := (iio pe).
 
-  Definition W := explicit_writes cd.
-  Definition R := explicit_reads cd.
-  Definition Wx := exclusive_writes cd.
-  Definition Rx := exclusive_writes cd.
-  Definition L := rel_acq_writes cd.
-  Definition A := rel_acq_reads cd.
-  Definition Q := acq_rcpc_reads cd.
-  Definition T := ttw_reads cd.
-
-  (* All cache flushing operations *)
-  Definition C := collect_all (λ _ ev, is_tlbop ev ∨ is_cacheop ev) cd.
-  Definition TLBI := collect_all (λ _ ev, is_tlbop ev) cd.
-  Definition TE := collect_all (λ _ event, is_take_exception event) cd.
-  Definition ERET := collect_all (λ _ event, is_return_exception event) cd.
+  (** ** Registers *)
+  Notation RR := (reg_reads pe).
+  Notation RW := (reg_writes pe).
+  Definition RE := RR ∪ RW.
+  Notation rrf := (reg_reads_from cd).
+  Notation rfr := (reg_from_reads cd).
 
   Definition is_msr := is_reg_writeP (λ _ o _, is_Some o).
   #[export] Typeclasses Transparent is_msr.
   Definition MSR := collect_all (λ _, is_msr) cd.
+  Definition is_mrs := is_reg_readP (λ _ o _, is_Some o).
+  #[export] Typeclasses Transparent is_mrs.
+  Definition MRS := collect_all (λ _, is_mrs) cd.
 
+  (** ** Barriers *)
+  Notation F := (barriers cd).
+  Notation ISB := (isb cd).
+
+  (** ** Memory *)
+  Notation W := (explicit_writes pe).
+  Notation R := (explicit_reads pe).
+  Notation M := (mem_explicit pe).
+  Notation Wx := (exclusive_writes pe).
+  Notation Rx := (exclusive_writes pe).
+  Notation L := (rel_acq_writes pe).
+  Notation A := (rel_acq_reads pe).
+  Notation Q := (acq_rcpc_reads pe).
+  Notation T := (ttw_reads pe).
+  Notation IF := (ifetch_reads pe).
+  Notation IR := (init_mem_reads cd).
+
+  Notation lxsx := (lxsx cd).
+  Notation amo := (atomic_update cd).
+  Definition rmw := lxsx ∪ amo.
+
+  (* Not necessarily transitive in mixed-size contexts *)
+  Definition co := ⦗W⦘⨾coherence cd⨾⦗W⦘ ∩ overlapping cd.
+  Definition coi := co ∩ int.
+  Definition coe := co ∖ coi.
+
+  Definition rf := reads_from cd⨾⦗R⦘.
+  Definition rfi := rf ∩ int.
+  Definition rfe := rf ∖ rfi.
+  Definition fr := ⦗R⦘⨾from_reads cd.
+  Definition fri := fr ∩ int.
+  Definition fre := fr ∖ fri.
+
+  Definition frf := fr⨾rf ∩ overlapping cd.
+  Definition frfi := frf ∩ int.
+
+  Definition trf := reads_from cd⨾⦗T⦘.
+  Definition trfi := trf ∩ int.
+  Definition trfe := trf ∖ rfi.
+  Definition tfr := ⦗T⦘⨾from_reads cd.
+  Definition tfri := tfr ∩ int.
+  Definition tfre := tfr ∖ fri.
+
+  Definition irf := reads_from cd⨾⦗IF⦘.
+  Definition irfi := irf ∩ int.
+  Definition irfe := irf ∖ rfi.
+  Definition ifr := ⦗IF⦘⨾from_reads cd.
+  Definition ifri := ifr ∩ int.
+  Definition ifre := ifr ∖ fri.
+
+
+
+  (** ** Caches *)
+  Definition ICDC := collect_all (λ _ ev, is_cacheop ev) cd.
+  Definition TLBI := collect_all (λ _ ev, is_tlbop ev) cd.
+  Definition C := ICDC ∪ TLBI.
+
+  (** ** Exceptions *)
+
+  Definition TE := collect_all (λ _ event, is_take_exception event) cd.
+  Definition ERET := collect_all (λ _ event, is_return_exception event) cd.
+
+  (** ** Explicit events *)
+
+  (** Explicit events are events that are the "main" event of an instruction
+
+      TODO: TE and ERET ? *)
+  Definition Exp := MRS ∪ MSR ∪ M ∪ F ∪ C.
+
+  Definition po := ⦗Exp⦘⨾instruction_order⨾⦗Exp⦘.
 
   (* A MemRead with ttw and value 0 *)
   Definition is_translation_read_fault :=
@@ -155,8 +229,65 @@ Module AxArmNames.
     set_unfold. hauto q:on use:is_mem_readP_spec.
   Qed.
 
-  Definition amo := atomic_update cd.
 
-  Definition rmw := lxsx cd ∪ amo.
+  (* #[export] Typeclasses Transparent not. *)
+
+  (** ** Internal coherence *)
+
+  (** Internal check for explicit accesses. This is equivalent to
+      grel_acyclic (po ∩ overlapping ∪ fr ∪ co ∪ rf) *)
+  Definition not_after := instruction_order ∪ (si ∖ iio⁻¹).
+  #[export] Typeclasses Transparent not_after.
+  (** Arm expresses their constraints as an irreflexive with po. This proves
+      the same by being included in [not_after] *)
+  Lemma not_after_spec_gen rel ov :
+    grel_symmetric ov →
+    rel ⊆ int ∩ ov → grel_irreflexive ((full_instruction_order ∩ ov)⨾ rel) ↔ rel ⊆ not_after.
+  Proof.
+    intros Hov Hin.
+    split.
+    - intros Ha [x y] Hrel.
+      apply NNPP. intro Hna.
+      set_unfold in Hna.
+      cdestruct Hna ##cdestruct_or.
+      1: assert ((y, x) ∈ instruction_order) by (set_unfold #UnfoldEidRels; hauto l:on).
+      all: set_solver.
+    - intros Hr x Hc.
+      set_unfold in Hc.
+      cdestruct Hc as y Hi Ho Hxyr.
+      set_unfold in Hr.
+      apply Hr in Hxyr.
+      intuition (set_unfold #UnfoldEidRels; lia).
+  Qed.
+
+  Lemma not_after_spec_po rel :
+    rel ⊆ int → grel_irreflexive (full_instruction_order⨾ rel) ↔ rel ⊆ not_after.
+  Proof.
+    intros Hin.
+    opose proof* (not_after_spec_gen rel int).
+    - set_solver#UnfoldEidRels.
+    - set_solver.
+    - by assert (full_instruction_order = full_instruction_order ∩ int)
+         as -> by set_solver#UnfoldEidRels.
+  Qed.
+  Definition not_after_spec_po_loc rel := not_after_spec_gen rel (overlapping cd) (overlapping_sym cd).
+
+  (** Statement of internal for explicit memory accesses. This ignores the
+  existence of implicit writes as none of our model allows them for now *)
+  Record exp_internal := {
+      rfi_internal : rfi ⊆ not_after; (* CoRW1: important, rfi not in ob *)
+      coi_internal : coi ⊆ not_after; (* CoWW: Also in ob via lws ∪ co*)
+      fri_internal : fri ⊆ not_after; (* CoWR0: Also in ob via lrs ∪ fr*)
+      frfi_internal : frfi ⊆ not_after; (* CoRR: important R;po-loc;R not in ob *)
+      (* CoRW2: not here as implied by ob (with co⨾rfe⨾lws) *)
+    }.
+
+  Record reg_internal := {
+      rrf_internal : rrf ⊆ full_instruction_order;
+      rfr_internal : rfr ⊆ not_after
+    }.
+
+
+
   End ArmNames.
 End AxArmNames.
